solve_by_elim garbage

src/cram.lean
@@ -1,4 +1,5 @@
 import tactic.suggest
+import tactic.solve_by_elim
 import data.nat.basic
 
 open tactic
@@ -30,10 +31,34 @@ meta def cram (discharger : tactic unit := done) : tactic string :=
 -- want recurse on cram so that to some depth, and if the goal is solved return the message
 -- just like library_search.
 
+open interactive lean.parser interactive.types
+open suggest
+local postfix `?`:9001 := optional
+
 namespace interactive
 
 meta def cram (discharger : tactic unit := done) : tactic unit :=
 tactic.cram >>= trace
+
+--This tactic is suppose to be a mix between suggest and solve_by_elim.
+--Solve_by_elim already works, just need it too print
+meta def baby_back (all_goals : parse $ (tk "*")?)
+ (no_dflt : parse only_flag)
+ (hs : parse simp_arg_list)
+ (attr_names : parse with_ident_list)
+ (opt : by_elim_opt := { }) : tactic unit :=
+
+--duplicate code
+do [g] ← get_goals <|> fail "FAIL!",
+
+   asms ← mk_assumption_set no_dflt hs attr_names,
+   tactic.solve_by_elim { all_goals := all_goals.is_some, assumptions := return asms, ..opt },
+
+   s ← read,
+   m ← tactic_statement g,
+   g ← instantiate_mvars g,
+
+   trace m
 
 end interactive
 
@@ -44,3 +69,14 @@ begin
   rw h,
   exact j,
 end
+
+variables {m n k : ℕ}
+
+theorem lt_of_sub_lt_sub_left : m - n < m - k → k < n :=
+lt_imp_lt_of_le_imp_le (nat.sub_le_sub_left _)
+
+example : m - n < m - k → k < n :=
+begin solve_by_elim [lt_imp_lt_of_le_imp_le, nat.sub_le_sub_left], end
+
+example : m - n < m - k → k < n :=
+begin baby_back [lt_imp_lt_of_le_imp_le, nat.sub_le_sub_left], end
